<?xml version="1.0"?>
<rdf:RDF xmlns="http://www.project-best.eu/owl/aixm#"
     xml:base="http://www.project-best.eu/owl/aixm"
     xmlns:rdf="http://www.w3.org/1999/02/22-rdf-syntax-ns#"
     xmlns:owl="http://www.w3.org/2002/07/owl#"
     xmlns:xsd="http://www.w3.org/2001/XMLSchema#"
     xmlns:rdfs="http://www.w3.org/2000/01/rdf-schema#"
     xmlns:aixm-geo="http://www.project-best.eu/owl/aixm-mod/geometry">
    <owl:Ontology rdf:about="http://www.project-best.eu/owl/aixm-mod/geometry"/>
    


    <!-- 
    ///////////////////////////////////////////////////////////////////////////////////////
    //
    // Object Properties
    //
    ///////////////////////////////////////////////////////////////////////////////////////
     -->

    


    <!-- http://www.project-best.eu/owl/aixm-mod/geometry#ElevatedCurve-verticalDatum -->

    <owl:ObjectProperty rdf:about="http://www.project-best.eu/owl/aixm-mod/geometry#ElevatedCurve-verticalDatum">
        <rdfs:comment xml:lang="en">The set of reference points or a mathematical model of the Earth&apos;s surface (a datum) against which vertical position measurements are made as basis for measuring elevations.</rdfs:comment>
        <rdfs:range rdf:resource="http://www.project-best.eu/owl/aixm-mod/geometry#CodeVerticalDatumType"/>
        <rdfs:domain rdf:resource="http://www.project-best.eu/owl/aixm-mod/geometry#ElevatedCurve"/>
        <rdfs:subPropertyOf rdf:resource="http://www.project-best.eu/owl/aixm-mod/geometry#ElevatedCurve_OP_"/>
    </owl:ObjectProperty>
    


    <!-- http://www.project-best.eu/owl/aixm-mod/geometry#ElevatedCurve_OP_ -->

    <owl:ObjectProperty rdf:about="http://www.project-best.eu/owl/aixm-mod/geometry#ElevatedCurve_OP_">
        <rdfs:subPropertyOf rdf:resource="http://www.project-best.eu/owl/aixm-mod/geometry#_Geometry_OP_"/>
    </owl:ObjectProperty>
    


    <!-- http://www.project-best.eu/owl/aixm-mod/geometry#ElevatedPoint-verticalDatum -->

    <owl:ObjectProperty rdf:about="http://www.project-best.eu/owl/aixm-mod/geometry#ElevatedPoint-verticalDatum">
        <rdfs:comment xml:lang="en">The set of reference points or a mathematical model of the Earth&apos;s surface (a datum) against which vertical position measurements are made as basis for measuring elevations.</rdfs:comment>
        <rdfs:range rdf:resource="http://www.project-best.eu/owl/aixm-mod/geometry#CodeVerticalDatumType"/>
        <rdfs:domain rdf:resource="http://www.project-best.eu/owl/aixm-mod/geometry#ElevatedPoint"/>
        <rdfs:subPropertyOf rdf:resource="http://www.project-best.eu/owl/aixm-mod/geometry#ElevatedPoint_OP_"/>
    </owl:ObjectProperty>
    


    <!-- http://www.project-best.eu/owl/aixm-mod/geometry#ElevatedPoint_OP_ -->

    <owl:ObjectProperty rdf:about="http://www.project-best.eu/owl/aixm-mod/geometry#ElevatedPoint_OP_">
        <rdfs:subPropertyOf rdf:resource="http://www.project-best.eu/owl/aixm-mod/geometry#_Geometry_OP_"/>
    </owl:ObjectProperty>
    


    <!-- http://www.project-best.eu/owl/aixm-mod/geometry#ElevatedSurface-verticalDatum -->

    <owl:ObjectProperty rdf:about="http://www.project-best.eu/owl/aixm-mod/geometry#ElevatedSurface-verticalDatum">
        <rdfs:comment xml:lang="en">The set of reference points or a mathematical model of the Earth&apos;s surface (a datum) against which vertical position measurements are made as basis for measuring elevations.</rdfs:comment>
        <rdfs:range rdf:resource="http://www.project-best.eu/owl/aixm-mod/geometry#CodeVerticalDatumType"/>
        <rdfs:domain rdf:resource="http://www.project-best.eu/owl/aixm-mod/geometry#ElevatedSurface"/>
        <rdfs:subPropertyOf rdf:resource="http://www.project-best.eu/owl/aixm-mod/geometry#ElevatedSurface_OP_"/>
    </owl:ObjectProperty>
    


    <!-- http://www.project-best.eu/owl/aixm-mod/geometry#ElevatedSurface_OP_ -->

    <owl:ObjectProperty rdf:about="http://www.project-best.eu/owl/aixm-mod/geometry#ElevatedSurface_OP_">
        <rdfs:subPropertyOf rdf:resource="http://www.project-best.eu/owl/aixm-mod/geometry#_Geometry_OP_"/>
    </owl:ObjectProperty>
    


    <!-- http://www.project-best.eu/owl/aixm-mod/geometry#_AIXMFeatures_OP_ -->

    <owl:ObjectProperty rdf:about="http://www.project-best.eu/owl/aixm-mod/geometry#_AIXMFeatures_OP_"/>
    


    <!-- http://www.project-best.eu/owl/aixm-mod/geometry#_Geometry_OP_ -->

    <owl:ObjectProperty rdf:about="http://www.project-best.eu/owl/aixm-mod/geometry#_Geometry_OP_">
        <rdfs:subPropertyOf rdf:resource="http://www.project-best.eu/owl/aixm-mod/geometry#_AIXMFeatures_OP_"/>
    </owl:ObjectProperty>
    


    <!-- 
    ///////////////////////////////////////////////////////////////////////////////////////
    //
    // Data properties
    //
    ///////////////////////////////////////////////////////////////////////////////////////
     -->

    


    <!-- http://www.project-best.eu/owl/aixm-mod/geometry#Curve-horizontalAccuracy -->

    <owl:DatatypeProperty rdf:about="http://www.project-best.eu/owl/aixm-mod/geometry#Curve-horizontalAccuracy">
        <rdfs:comment xml:lang="en">The difference between the recorded horizontal coordinates of a feature and its true position referenced to the same geodetic datum expressed as a circular error at 95 percent probability.</rdfs:comment>
        <rdfs:domain rdf:resource="http://www.project-best.eu/owl/aixm-mod/geometry#Curve"/>
        <rdfs:subPropertyOf rdf:resource="http://www.project-best.eu/owl/aixm-mod/geometry#Curve_DP_"/>
        <rdfs:range rdf:resource="http://www.w3.org/2001/XMLSchema#decimal"/>
    </owl:DatatypeProperty>
    


    <!-- http://www.project-best.eu/owl/aixm-mod/geometry#Curve_DP_ -->

    <owl:DatatypeProperty rdf:about="http://www.project-best.eu/owl/aixm-mod/geometry#Curve_DP_">
        <rdfs:subPropertyOf rdf:resource="http://www.project-best.eu/owl/aixm-mod/geometry#_Geometry_DP_"/>
    </owl:DatatypeProperty>
    


    <!-- http://www.project-best.eu/owl/aixm-mod/geometry#ElevatedCurve-elevation -->

    <owl:DatatypeProperty rdf:about="http://www.project-best.eu/owl/aixm-mod/geometry#ElevatedCurve-elevation">
        <rdfs:comment xml:lang="en">The vertical distance at the curve level, measured from Mean Sea Level (MSL).</rdfs:comment>
        <rdfs:domain rdf:resource="http://www.project-best.eu/owl/aixm-mod/geometry#ElevatedCurve"/>
        <rdfs:subPropertyOf rdf:resource="http://www.project-best.eu/owl/aixm-mod/geometry#ElevatedCurve_DP_"/>
        <rdfs:range rdf:resource="http://www.w3.org/2001/XMLSchema#decimal"/>
    </owl:DatatypeProperty>
    


    <!-- http://www.project-best.eu/owl/aixm-mod/geometry#ElevatedCurve-geoidUndulation -->

    <owl:DatatypeProperty rdf:about="http://www.project-best.eu/owl/aixm-mod/geometry#ElevatedCurve-geoidUndulation">
        <rdfs:comment xml:lang="en">The distance of the geoid above (positive) or below (negative) the mathematical reference ellipsoid at the location of the curve.</rdfs:comment>
        <rdfs:domain rdf:resource="http://www.project-best.eu/owl/aixm-mod/geometry#ElevatedCurve"/>
        <rdfs:subPropertyOf rdf:resource="http://www.project-best.eu/owl/aixm-mod/geometry#ElevatedCurve_DP_"/>
        <rdfs:range rdf:resource="http://www.w3.org/2001/XMLSchema#decimal"/>
    </owl:DatatypeProperty>
    


    <!-- http://www.project-best.eu/owl/aixm-mod/geometry#ElevatedCurve-verticalAccuracy -->

    <owl:DatatypeProperty rdf:about="http://www.project-best.eu/owl/aixm-mod/geometry#ElevatedCurve-verticalAccuracy">
        <rdfs:comment xml:lang="en">The difference between the recorded elevation of a feature and its true elevation referenced to the same vertical datum expressed as a linear error at 95 percent probability.</rdfs:comment>
        <rdfs:domain rdf:resource="http://www.project-best.eu/owl/aixm-mod/geometry#ElevatedCurve"/>
        <rdfs:subPropertyOf rdf:resource="http://www.project-best.eu/owl/aixm-mod/geometry#ElevatedCurve_DP_"/>
        <rdfs:range rdf:resource="http://www.w3.org/2001/XMLSchema#decimal"/>
    </owl:DatatypeProperty>
    


    <!-- http://www.project-best.eu/owl/aixm-mod/geometry#ElevatedCurve_DP_ -->

    <owl:DatatypeProperty rdf:about="http://www.project-best.eu/owl/aixm-mod/geometry#ElevatedCurve_DP_">
        <rdfs:subPropertyOf rdf:resource="http://www.project-best.eu/owl/aixm-mod/geometry#_Geometry_DP_"/>
    </owl:DatatypeProperty>
    


    <!-- http://www.project-best.eu/owl/aixm-mod/geometry#ElevatedPoint-elevation -->

    <owl:DatatypeProperty rdf:about="http://www.project-best.eu/owl/aixm-mod/geometry#ElevatedPoint-elevation">
        <rdfs:comment xml:lang="en">The vertical distance of the point measured from Mean Sea Level (MSL).</rdfs:comment>
        <rdfs:domain rdf:resource="http://www.project-best.eu/owl/aixm-mod/geometry#ElevatedPoint"/>
        <rdfs:subPropertyOf rdf:resource="http://www.project-best.eu/owl/aixm-mod/geometry#ElevatedPoint_DP_"/>
        <rdfs:range rdf:resource="http://www.w3.org/2001/XMLSchema#decimal"/>
    </owl:DatatypeProperty>
    


    <!-- http://www.project-best.eu/owl/aixm-mod/geometry#ElevatedPoint-geoidUndulation -->

    <owl:DatatypeProperty rdf:about="http://www.project-best.eu/owl/aixm-mod/geometry#ElevatedPoint-geoidUndulation">
        <rdfs:comment xml:lang="en">The distance of the geoid above (positive) or below (negative) the mathematical reference ellipsoid at the location of the point.</rdfs:comment>
        <rdfs:domain rdf:resource="http://www.project-best.eu/owl/aixm-mod/geometry#ElevatedPoint"/>
        <rdfs:subPropertyOf rdf:resource="http://www.project-best.eu/owl/aixm-mod/geometry#ElevatedPoint_DP_"/>
        <rdfs:range rdf:resource="http://www.w3.org/2001/XMLSchema#decimal"/>
    </owl:DatatypeProperty>
    


    <!-- http://www.project-best.eu/owl/aixm-mod/geometry#ElevatedPoint-verticalAccuracy -->

    <owl:DatatypeProperty rdf:about="http://www.project-best.eu/owl/aixm-mod/geometry#ElevatedPoint-verticalAccuracy">
        <rdfs:comment xml:lang="en">The difference between the recorded elevation of a feature and its true elevation referenced to the same vertical datum expressed as a linear error at 95 percent probability.</rdfs:comment>
        <rdfs:domain rdf:resource="http://www.project-best.eu/owl/aixm-mod/geometry#ElevatedPoint"/>
        <rdfs:subPropertyOf rdf:resource="http://www.project-best.eu/owl/aixm-mod/geometry#ElevatedPoint_DP_"/>
        <rdfs:range rdf:resource="http://www.w3.org/2001/XMLSchema#decimal"/>
    </owl:DatatypeProperty>
    


    <!-- http://www.project-best.eu/owl/aixm-mod/geometry#ElevatedPoint_DP_ -->

    <owl:DatatypeProperty rdf:about="http://www.project-best.eu/owl/aixm-mod/geometry#ElevatedPoint_DP_">
        <rdfs:subPropertyOf rdf:resource="http://www.project-best.eu/owl/aixm-mod/geometry#_Geometry_DP_"/>
    </owl:DatatypeProperty>
    


    <!-- http://www.project-best.eu/owl/aixm-mod/geometry#ElevatedSurface-elevation -->

    <owl:DatatypeProperty rdf:about="http://www.project-best.eu/owl/aixm-mod/geometry#ElevatedSurface-elevation">
        <rdfs:comment xml:lang="en">The vertical distance of the surface level measured from Mean Sea Level (MSL).</rdfs:comment>
        <rdfs:domain rdf:resource="http://www.project-best.eu/owl/aixm-mod/geometry#ElevatedSurface"/>
        <rdfs:subPropertyOf rdf:resource="http://www.project-best.eu/owl/aixm-mod/geometry#ElevatedSurface_DP_"/>
        <rdfs:range rdf:resource="http://www.w3.org/2001/XMLSchema#decimal"/>
    </owl:DatatypeProperty>
    


    <!-- http://www.project-best.eu/owl/aixm-mod/geometry#ElevatedSurface-geoidUndulation -->

    <owl:DatatypeProperty rdf:about="http://www.project-best.eu/owl/aixm-mod/geometry#ElevatedSurface-geoidUndulation">
        <rdfs:comment xml:lang="en">The distance of the geoid above (positive) or below (negative) the mathematical reference ellipsoid at the location of the surface.</rdfs:comment>
        <rdfs:domain rdf:resource="http://www.project-best.eu/owl/aixm-mod/geometry#ElevatedSurface"/>
        <rdfs:subPropertyOf rdf:resource="http://www.project-best.eu/owl/aixm-mod/geometry#ElevatedSurface_DP_"/>
        <rdfs:range rdf:resource="http://www.w3.org/2001/XMLSchema#decimal"/>
    </owl:DatatypeProperty>
    


    <!-- http://www.project-best.eu/owl/aixm-mod/geometry#ElevatedSurface-verticalAccuracy -->

    <owl:DatatypeProperty rdf:about="http://www.project-best.eu/owl/aixm-mod/geometry#ElevatedSurface-verticalAccuracy">
        <rdfs:comment xml:lang="en">The difference between the recorded elevation of a feature and its true elevation referenced to the same vertical datum expressed as a linear error at 95 percent probability.</rdfs:comment>
        <rdfs:domain rdf:resource="http://www.project-best.eu/owl/aixm-mod/geometry#ElevatedSurface"/>
        <rdfs:subPropertyOf rdf:resource="http://www.project-best.eu/owl/aixm-mod/geometry#ElevatedSurface_DP_"/>
        <rdfs:range rdf:resource="http://www.w3.org/2001/XMLSchema#decimal"/>
    </owl:DatatypeProperty>
    


    <!-- http://www.project-best.eu/owl/aixm-mod/geometry#ElevatedSurface_DP_ -->

    <owl:DatatypeProperty rdf:about="http://www.project-best.eu/owl/aixm-mod/geometry#ElevatedSurface_DP_">
        <rdfs:subPropertyOf rdf:resource="http://www.project-best.eu/owl/aixm-mod/geometry#_Geometry_DP_"/>
    </owl:DatatypeProperty>
    


    <!-- http://www.project-best.eu/owl/aixm-mod/geometry#Point-horizontalAccuracy -->

    <owl:DatatypeProperty rdf:about="http://www.project-best.eu/owl/aixm-mod/geometry#Point-horizontalAccuracy">
        <rdfs:comment xml:lang="en">The difference between the recorded horizontal coordinates of a feature and its true position referenced to the same geodetic datum expressed as a circular error at 95 percent probability.</rdfs:comment>
        <rdfs:domain rdf:resource="http://www.project-best.eu/owl/aixm-mod/geometry#Point"/>
        <rdfs:subPropertyOf rdf:resource="http://www.project-best.eu/owl/aixm-mod/geometry#Point_DP_"/>
        <rdfs:range rdf:resource="http://www.w3.org/2001/XMLSchema#decimal"/>
    </owl:DatatypeProperty>
    


    <!-- http://www.project-best.eu/owl/aixm-mod/geometry#Point_DP_ -->

    <owl:DatatypeProperty rdf:about="http://www.project-best.eu/owl/aixm-mod/geometry#Point_DP_">
        <rdfs:subPropertyOf rdf:resource="http://www.project-best.eu/owl/aixm-mod/geometry#_Geometry_DP_"/>
    </owl:DatatypeProperty>
    


    <!-- http://www.project-best.eu/owl/aixm-mod/geometry#Surface-horizontalAccuracy -->

    <owl:DatatypeProperty rdf:about="http://www.project-best.eu/owl/aixm-mod/geometry#Surface-horizontalAccuracy">
        <rdfs:comment xml:lang="en">The difference between the recorded horizontal coordinates of a feature and its true position referenced to the same geodetic datum expressed as a circular error at 95 percent probability.</rdfs:comment>
        <rdfs:domain rdf:resource="http://www.project-best.eu/owl/aixm-mod/geometry#Surface"/>
        <rdfs:subPropertyOf rdf:resource="http://www.project-best.eu/owl/aixm-mod/geometry#Surface_DP_"/>
        <rdfs:range rdf:resource="http://www.w3.org/2001/XMLSchema#decimal"/>
    </owl:DatatypeProperty>
    


    <!-- http://www.project-best.eu/owl/aixm-mod/geometry#Surface_DP_ -->

    <owl:DatatypeProperty rdf:about="http://www.project-best.eu/owl/aixm-mod/geometry#Surface_DP_">
        <rdfs:subPropertyOf rdf:resource="http://www.project-best.eu/owl/aixm-mod/geometry#_Geometry_DP_"/>
    </owl:DatatypeProperty>
    


    <!-- http://www.project-best.eu/owl/aixm-mod/geometry#_Geometry_DP_ -->

    <owl:DatatypeProperty rdf:about="http://www.project-best.eu/owl/aixm-mod/geometry#_Geometry_DP_"/>
    


    <!-- 
    ///////////////////////////////////////////////////////////////////////////////////////
    //
    // Classes
    //
    ///////////////////////////////////////////////////////////////////////////////////////
     -->

    


    <!-- http://www.project-best.eu/owl/aixm-mod/geometry#CodeVerticalDatumType -->

    <owl:Class rdf:about="http://www.project-best.eu/owl/aixm-mod/geometry#CodeVerticalDatumType">
        <rdfs:subClassOf rdf:resource="http://www.project-best.eu/owl/aixm-mod/geometry#_Codelists_"/>
        <rdfs:comment xml:lang="en">List of vertical datums.</rdfs:comment>
    </owl:Class>
    


    <!-- http://www.project-best.eu/owl/aixm-mod/geometry#Curve -->

    <owl:Class rdf:about="http://www.project-best.eu/owl/aixm-mod/geometry#Curve">
        <rdfs:subClassOf rdf:resource="http://www.project-best.eu/owl/aixm-mod/geometry#_Geometry_"/>
        <rdfs:comment xml:lang="en">An AIXM curve derived from GM_Curve and extended to include Horizontal Accuracy Properties</rdfs:comment>
    </owl:Class>
    


    <!-- http://www.project-best.eu/owl/aixm-mod/geometry#ElevatedCurve -->

    <owl:Class rdf:about="http://www.project-best.eu/owl/aixm-mod/geometry#ElevatedCurve">
        <rdfs:subClassOf rdf:resource="http://www.project-best.eu/owl/aixm-mod/geometry#Curve"/>
        <rdfs:comment xml:lang="en">An AIXM elevated curve derived from, which extends curve with properties that represent the vertical position (elevation, datum, accuracy).</rdfs:comment>
    </owl:Class>
    


    <!-- http://www.project-best.eu/owl/aixm-mod/geometry#ElevatedPoint -->

    <owl:Class rdf:about="http://www.project-best.eu/owl/aixm-mod/geometry#ElevatedPoint">
        <rdfs:subClassOf rdf:resource="http://www.project-best.eu/owl/aixm-mod/geometry#Point"/>
        <rdfs:comment xml:lang="en">An AIXM Point derived from GM_Point that includes properties for describing a point with elevation and vertical extent.  Used in obstacles, navaids, etc.</rdfs:comment>
    </owl:Class>
    


    <!-- http://www.project-best.eu/owl/aixm-mod/geometry#ElevatedSurface -->

    <owl:Class rdf:about="http://www.project-best.eu/owl/aixm-mod/geometry#ElevatedSurface">
        <rdfs:subClassOf rdf:resource="http://www.project-best.eu/owl/aixm-mod/geometry#Surface"/>
        <rdfs:comment xml:lang="en">An AIXM elevated surface derived from, which extends Surface with properties that represent the vertical position (elevation, datum, accuracy).</rdfs:comment>
    </owl:Class>
    


    <!-- http://www.project-best.eu/owl/aixm-mod/geometry#Point -->

    <owl:Class rdf:about="http://www.project-best.eu/owl/aixm-mod/geometry#Point">
        <rdfs:subClassOf rdf:resource="http://www.project-best.eu/owl/aixm-mod/geometry#_Geometry_"/>
        <rdfs:comment xml:lang="en">AIXM Point containing horizontal accuracy data. In AIXM horizontal accuracy is considered a property of the geometry.</rdfs:comment>
    </owl:Class>
    


    <!-- http://www.project-best.eu/owl/aixm-mod/geometry#Surface -->

    <owl:Class rdf:about="http://www.project-best.eu/owl/aixm-mod/geometry#Surface">
        <rdfs:subClassOf rdf:resource="http://www.project-best.eu/owl/aixm-mod/geometry#_Geometry_"/>
        <rdfs:comment xml:lang="en">An AIXM surface derived from GM_Surface and extended to include Horizontal Accuracy Properties</rdfs:comment>
    </owl:Class>
    


    <!-- http://www.project-best.eu/owl/aixm-mod/geometry#_AIXMDataTypes_ -->

    <owl:Class rdf:about="http://www.project-best.eu/owl/aixm-mod/geometry#_AIXMDataTypes_">
        <rdfs:comment xml:lang="en">The complex datatypes used by AIXM are changed to simple data
            types, so only the codelists are represented within the _AIXMDataTypes_
            package/class.</rdfs:comment>
    </owl:Class>
    


    <!-- http://www.project-best.eu/owl/aixm-mod/geometry#_AIXMFeatures_ -->

    <owl:Class rdf:about="http://www.project-best.eu/owl/aixm-mod/geometry#_AIXMFeatures_"/>
    


    <!-- http://www.project-best.eu/owl/aixm-mod/geometry#_Codelists_ -->

    <owl:Class rdf:about="http://www.project-best.eu/owl/aixm-mod/geometry#_Codelists_">
        <rdfs:subClassOf rdf:resource="http://www.project-best.eu/owl/aixm-mod/geometry#_AIXMDataTypes_"/>
    </owl:Class>
    


    <!-- http://www.project-best.eu/owl/aixm-mod/geometry#_Geometry_ -->

    <owl:Class rdf:about="http://www.project-best.eu/owl/aixm-mod/geometry#_Geometry_">
        <rdfs:subClassOf rdf:resource="http://www.project-best.eu/owl/aixm-mod/geometry#_AIXMFeatures_"/>
    </owl:Class>
    


    <!-- 
    ///////////////////////////////////////////////////////////////////////////////////////
    //
    // Individuals
    //
    ///////////////////////////////////////////////////////////////////////////////////////
     -->

    


    <!-- http://www.project-best.eu/owl/aixm-mod/geometry#CodeVerticalDatumBaseType-AHD -->

    <owl:NamedIndividual rdf:about="http://www.project-best.eu/owl/aixm-mod/geometry#CodeVerticalDatumBaseType-AHD">
        <rdf:type rdf:resource="http://www.project-best.eu/owl/aixm-mod/geometry#CodeVerticalDatumType"/>
        <rdfs:comment xml:lang="en">Australian Height Datum</rdfs:comment>
    </owl:NamedIndividual>
    


    <!-- http://www.project-best.eu/owl/aixm-mod/geometry#CodeVerticalDatumBaseType-EGM_96 -->

    <owl:NamedIndividual rdf:about="http://www.project-best.eu/owl/aixm-mod/geometry#CodeVerticalDatumBaseType-EGM_96">
        <rdf:type rdf:resource="http://www.project-best.eu/owl/aixm-mod/geometry#CodeVerticalDatumType"/>
        <rdfs:comment xml:lang="en">(ICAO Doc 9674) Earth gravitational model 1996.  ICAO recommended vertical datum.</rdfs:comment>
    </owl:NamedIndividual>
    


    <!-- http://www.project-best.eu/owl/aixm-mod/geometry#CodeVerticalDatumBaseType-NAVD88 -->

    <owl:NamedIndividual rdf:about="http://www.project-best.eu/owl/aixm-mod/geometry#CodeVerticalDatumBaseType-NAVD88">
        <rdf:type rdf:resource="http://www.project-best.eu/owl/aixm-mod/geometry#CodeVerticalDatumType"/>
        <rdfs:comment xml:lang="en">North American Vertical Datum of 1988</rdfs:comment>
    </owl:NamedIndividual>
    


    <!-- http://www.project-best.eu/owl/aixm-mod/geometry#CodeVerticalDatumBaseType-OTHER -->

    <owl:NamedIndividual rdf:about="http://www.project-best.eu/owl/aixm-mod/geometry#CodeVerticalDatumBaseType-OTHER">
        <rdf:type rdf:resource="http://www.project-best.eu/owl/aixm-mod/geometry#CodeVerticalDatumType"/>
        <rdfs:comment xml:lang="en">Other</rdfs:comment>
    </owl:NamedIndividual>
</rdf:RDF>



<!-- Generated by the OWL API (version 1.3.8.1099) http://owlapi.sourceforge.net -->

